src/theorems/safety.lean
@@ -42,7 +42,7 @@ begin
   cases arrow_canonical_forms h et_a,
   cases h_2,
   right,
-  existsi subst et_e2 w h_2_w emp.right,
+  existsi subst et_e2 w emp.right h_2_w,
   let d := @steps.app_done w et_τ1 h_2_w et_e2 emp.right h_1,
   -- avoid weird 'motive is not type correct' error
   rw symm h_2_h at d,
